<?xml version="1.0"?>
<rdf:RDF xmlns="http://emmo.info/emmo/middle/holistic#"
     xml:base="http://emmo.info/emmo/middle/holistic"
     xmlns:owl="http://www.w3.org/2002/07/owl#"
     xmlns:rdf="http://www.w3.org/1999/02/22-rdf-syntax-ns#"
     xmlns:xml="http://www.w3.org/XML/1998/namespace"
     xmlns:xsd="http://www.w3.org/2001/XMLSchema#"
     xmlns:rdfs="http://www.w3.org/2000/01/rdf-schema#"
     xmlns:annotations="http://emmo.info/emmo/top/annotations#">
    <owl:Ontology rdf:about="http://emmo.info/emmo/middle/holistic">
        <owl:versionIRI rdf:resource="http://emmo.info/emmo/1.0.0-alpha2/middle/holistic"/>
        <owl:imports rdf:resource="http://emmo.info/emmo/1.0.0-alpha2/top"/>
        <annotations:EMMO_5525a055_dda5_4556_8b91_f0d22fa676cc>EMMO is released under a Creative Commons license Attribution 4.0 International (CC BY 4.0)

https://creativecommons.org/licenses/by/4.0/legalcode</annotations:EMMO_5525a055_dda5_4556_8b91_f0d22fa676cc>
        <annotations:EMMO_cd5fb112_7ee7_4120_a35d_3ca3e6c3f4ab>Emanuele Ghedini (University of Bologna, IT)
Gerhard Goldbeck (GCL Ltd, UK)
Adham Hashibon (Fraunhofer IWM, DE)
Georg Schmitz (Access, DE)
Jesper Friis (SINTEF, NO)</annotations:EMMO_cd5fb112_7ee7_4120_a35d_3ca3e6c3f4ab>
        <rdfs:comment>Contacts:
Gerhard Goldbeck
Goldbeck Consulting Ltd (UK)
email: gerhard@goldbeck-consulting.com

Emanuele Ghedini
University of Bologna (IT)
email: emanuele.ghedini</rdfs:comment>
        <rdfs:comment>European Materials and Modelling Ontology (EMMO)

EMMO is a multidisciplinary effort to develop a standard representational framework (the ontology) based on current materials modelling knowledge, including physical sciences, analytical philosophy and information and communication technologies. 

It provides the connection between the physical world, materials characterisation world and materials modelling world.</rdfs:comment>
        <rdfs:comment>The EMMO requires FacT++ reasoner plugin in order to visualize all inferences and class hierarchy (ctrl+R hotkey in Protege).</rdfs:comment>
        <owl:versionInfo>The European Materials Modelling Ontology

Version 1.0.0-alpha2</owl:versionInfo>
    </owl:Ontology>
    


    <!-- 
    ///////////////////////////////////////////////////////////////////////////////////////
    //
    // Object Properties
    //
    ///////////////////////////////////////////////////////////////////////////////////////
     -->

    


    <!-- http://emmo.info/emmo/middle/holistic#EMMO_ae2d1a96_bfa1_409a_a7d2_03d69e8a125a -->

    <owl:ObjectProperty rdf:about="http://emmo.info/emmo/middle/holistic#EMMO_ae2d1a96_bfa1_409a_a7d2_03d69e8a125a">
        <rdfs:subPropertyOf rdf:resource="http://emmo.info/emmo/top/mereotopology#EMMO_17e27c22_37e1_468c_9dd7_95e137f73e7f"/>
        <rdfs:domain rdf:resource="http://emmo.info/emmo/middle/holistic#EMMO_43e9a05d_98af_41b4_92f6_00f79a09bfce"/>
        <rdfs:range rdf:resource="http://emmo.info/emmo/middle/holistic#EMMO_49804605_c0fe_4538_abda_f70ba1dc8a5d"/>
        <annotations:EMMO_967080e5_2f42_4eb2_a3a9_c58143e835f9>The relation between a process and an object participating to it.</annotations:EMMO_967080e5_2f42_4eb2_a3a9_c58143e835f9>
        <rdfs:comment>Participation is a parthood relation: you must be part (and then be connected) of the process to contribute to it.</rdfs:comment>
        <rdfs:comment>Participation is not under direct parthood since a process is not strictly related to reductionism, but it&apos;s a way to categorize temporal regions by the interpreters.</rdfs:comment>
        <rdfs:label xml:lang="en">hasParticipant</rdfs:label>
    </owl:ObjectProperty>
    


    <!-- http://emmo.info/emmo/middle/holistic#EMMO_c5aae418_1622_4d02_93c5_21159e28e6c1 -->

    <owl:ObjectProperty rdf:about="http://emmo.info/emmo/middle/holistic#EMMO_c5aae418_1622_4d02_93c5_21159e28e6c1">
        <rdfs:subPropertyOf rdf:resource="http://emmo.info/emmo/middle/holistic#EMMO_ae2d1a96_bfa1_409a_a7d2_03d69e8a125a"/>
        <rdfs:subPropertyOf rdf:resource="http://emmo.info/emmo/top/mereotopology#EMMO_9380ab64_0363_4804_b13f_3a8a94119a76"/>
        <rdfs:label xml:lang="en">hasProperParticipant</rdfs:label>
    </owl:ObjectProperty>
    


    <!-- 
    ///////////////////////////////////////////////////////////////////////////////////////
    //
    // Classes
    //
    ///////////////////////////////////////////////////////////////////////////////////////
     -->

    


    <!-- http://emmo.info/emmo/middle/holistic#EMMO_0277f24a_ea7f_4917_81b7_fb0406c8fc62 -->

    <owl:Class rdf:about="http://emmo.info/emmo/middle/holistic#EMMO_0277f24a_ea7f_4917_81b7_fb0406c8fc62">
        <owl:equivalentClass>
            <owl:Class>
                <owl:unionOf rdf:parseType="Collection">
                    <rdf:Description rdf:about="http://emmo.info/emmo/middle/holistic#EMMO_43e9a05d_98af_41b4_92f6_00f79a09bfce"/>
                    <rdf:Description rdf:about="http://emmo.info/emmo/middle/holistic#EMMO_49804605_c0fe_4538_abda_f70ba1dc8a5d"/>
                </owl:unionOf>
            </owl:Class>
        </owl:equivalentClass>
        <rdfs:subClassOf rdf:resource="http://emmo.info/emmo/top#EMMO_49267eba_5548_4163_8f36_518d65b583f9"/>
        <annotations:EMMO_967080e5_2f42_4eb2_a3a9_c58143e835f9>A union of classes that categorize physicals under a holistic perspective: the interest is on the whole 4D object (process) and the role of its 4D parts (participants) without going further into specifying the spatial hierarchy or the temporal position of each part.</annotations:EMMO_967080e5_2f42_4eb2_a3a9_c58143e835f9>
        <rdfs:comment>An holistic perspective considers each part of the whole as equally important, without the need of a granularity hierarchy (in time or space).

A molecule of a body can have role in the body evolution, without caring if its part of a specific organ and without specifying the time interval in which this role occurred.

This class allows the picking of parts without necessarily going trough a rigid hierarchy of spatial compositions (e.g. body -&gt; organ -&gt; cell -&gt; molecule) or temporal composition.</rdfs:comment>
        <rdfs:comment>Holism (from Greek ὅλος holos &quot;all, whole, entire&quot;)</rdfs:comment>
        <rdfs:label xml:lang="en">Holistic</rdfs:label>
    </owl:Class>
    


    <!-- http://emmo.info/emmo/middle/holistic#EMMO_43e9a05d_98af_41b4_92f6_00f79a09bfce -->

    <owl:Class rdf:about="http://emmo.info/emmo/middle/holistic#EMMO_43e9a05d_98af_41b4_92f6_00f79a09bfce">
        <rdfs:subClassOf rdf:resource="http://emmo.info/emmo/top/physical#EMMO_c5ddfdba_c074_4aa4_ad6b_1ac4942d300d"/>
        <rdfs:subClassOf>
            <owl:Restriction>
                <owl:onProperty rdf:resource="http://emmo.info/emmo/middle/holistic#EMMO_ae2d1a96_bfa1_409a_a7d2_03d69e8a125a"/>
                <owl:someValuesFrom rdf:resource="http://emmo.info/emmo/middle/holistic#EMMO_49804605_c0fe_4538_abda_f70ba1dc8a5d"/>
            </owl:Restriction>
        </rdfs:subClassOf>
        <annotations:EMMO_967080e5_2f42_4eb2_a3a9_c58143e835f9>A temporal part of a &apos;physical&apos; that identifies a particular type of evolution in time.</annotations:EMMO_967080e5_2f42_4eb2_a3a9_c58143e835f9>
        <rdfs:comment>A &apos;Process&apos; is always a &apos;Physical&apos;, since a &apos;Void&apos; does not have elements that evolves in time.</rdfs:comment>
        <rdfs:comment>Following the common definition of process, the reader may think that every &apos;Physical&apos; should be a process, since every 4D object always has a time dimension. 

However, in the EMMO we restrict the meaning of the word process to &apos;Physical&apos;-s whose evolution in time have a particular meaning for the ontologist (i.e. every 4D object unfolds in time, but not every 4D object may be of interest for the ontologist). 

A &apos;Process&apos; is not only something that unfolds in time (which is automatically represented in a 4D ontology), but something that has a meaning for the ontologist (i.e. that the ontologist can separate from the rest of the 4D physical for any reason).</rdfs:comment>
        <rdfs:label xml:lang="en">Process</rdfs:label>
    </owl:Class>
    


    <!-- http://emmo.info/emmo/middle/holistic#EMMO_49804605_c0fe_4538_abda_f70ba1dc8a5d -->

    <owl:Class rdf:about="http://emmo.info/emmo/middle/holistic#EMMO_49804605_c0fe_4538_abda_f70ba1dc8a5d">
        <rdfs:subClassOf rdf:resource="http://emmo.info/emmo/top/physical#EMMO_c5ddfdba_c074_4aa4_ad6b_1ac4942d300d"/>
        <rdfs:subClassOf>
            <owl:Restriction>
                <owl:onProperty>
                    <rdf:Description>
                        <owl:inverseOf rdf:resource="http://emmo.info/emmo/middle/holistic#EMMO_ae2d1a96_bfa1_409a_a7d2_03d69e8a125a"/>
                    </rdf:Description>
                </owl:onProperty>
                <owl:someValuesFrom rdf:resource="http://emmo.info/emmo/middle/holistic#EMMO_43e9a05d_98af_41b4_92f6_00f79a09bfce"/>
            </owl:Restriction>
        </rdfs:subClassOf>
        <annotations:EMMO_967080e5_2f42_4eb2_a3a9_c58143e835f9>A portion of a &apos;Process&apos; that participates to the process with a specific role.</annotations:EMMO_967080e5_2f42_4eb2_a3a9_c58143e835f9>
        <rdfs:comment>In the EMMO the relation of participation to a process falls under mereotopology.

Since topological connection means causality, then the only way for a real world object to participate to a process is to be a part of it.</rdfs:comment>
        <rdfs:label xml:lang="en">Participant</rdfs:label>
    </owl:Class>
</rdf:RDF>



<!-- Generated by the OWL API (version 4.5.9.2019-02-01T07:24:44Z) https://github.com/owlcs/owlapi -->

